Support for Curve25519.secret_to_public

specs/Spec.Curve25519.fst
@@ -5,8 +5,10 @@ open Lib.IntTypes
 open Lib.RawIntTypes
 open Lib.Sequence
 open Lib.ByteSequence
-open Spec.Curve25519.Lemmas
 open Lib.NatMod
+
+open Spec.Curve25519.Lemmas
+
 
 #reset-options "--max_fuel 0 --z3rlimit 20"
 
@@ -86,3 +88,9 @@ let scalarmult' (k:scalar) (u:serialized_point) : Tot serialized_point =
   let u = decodePoint u in
   let res = montgomery_ladder u k in
   encodePoint res
+
+val secret_to_public: lbytes 32 -> Tot (lbytes 32)
+let secret_to_public kpriv =
+  let basepoint_zeros = create 32 (u8 0) in
+  let basepoint = upd basepoint_zeros (32 - 1) (u8 0x09) in
+  scalarmult kpriv basepoint
